21. Derivatives

1.Compute derivatives of functions:

1. $y(x) = -3x + 3$

 derivative of \( y(x) = -3x + 3 \)

---

# Derivative of \( y(x) = -3x + 3 \)

\[
y(x) = -3x + 3
\]

### Solution

To find the derivative of $ y(x) $, we use the **basic derivative rules**:

1. The derivative of a constant $( c $) is $ 0 $:
   $$
   \frac{d}{dx}[c] = 0
   $$

2. The derivative of $ kx $, where $ k $ is a constant, is $$ k $$:
   $$
   \frac{d}{dx}[kx] = k
   $$

Applying these rules to $ y(x) = -3x + 3 $:

$$
\frac{dy}{dx} = \frac{d}{dx}[-3x] + \frac{d}{dx}[3]
$$

#### Step 1: Differentiate each term

- For the term $ -3x $:
  $$
  \frac{d}{dx}[-3x] = -3
  $$

- For the constant term $ 3 $:
  $$
  \frac{d}{dx}[3] = 0
  $$

#### Step 2: Combine the results
$$
\frac{dy}{dx} = -3 + 0 = -3
$$

### Final Answer

The derivative of $ y(x) = -3x + 3 $ is:

$$
\boxed{\frac{dy}{dx} = -3}
$$

---

### Explanation of the Result

1. The term $ -3x $ contributes a slope of $ -3 $, which means that the rate of change of $ y(x) $ with respect to $ x $ is constant and equal to $ -3 $.
2. The constant $ 3 $ has no effect on the slope because its derivative is $ 0 $.

This result tells us that the function $ y(x) $ is a straight line with a constant slope of $ -3 $.

---

2. $$y(x) = \pi x + sin(1)$$

To compute the derivative of $ y(x) = \pi x + \sin(1) $:

### Step 1: Break down the function
The function can be expressed as:
$$
y(x) = \pi x + \sin(1)
$$
- The term $ \pi x $ is a linear term.
- $ \sin(1) $ is a constant because $ 1 $ is independent of $ x $.

### Step 2: Derivative rules
- The derivative of $ \pi x $ with respect to $ x $ is $ \pi $ (since $\pi$ is a constant).
- The derivative of a constant ($ \sin(1) $) is $ 0 $.

### Step 3: Compute the derivative
$$
\frac{dy}{dx} = \pi + 0 = \pi
$$

### Final Answer
The derivative of $ y(x) = \pi x + \sin(1) $ is:
$$
\frac{dy}{dx} = \pi
$$

---

3. $$y(x) = 4 + sin(2)$$

To compute the derivative of $ y(x) = 4 + \sin(2) $:

### Step 1: Analyze the function
The given function is:
$
y(x) = 4 + \sin(2)
$
- $ 4 $ is a constant.
- $ \sin(2) $ is also a constant since $ 2 $ is independent of $ x $.

### Step 2: Derivative rules
- The derivative of a constant is $ 0 $.

### Step 3: Compute the derivative
$$
\frac{dy}{dx} = 0 + 0 = 0
$$

### Final Answer
The derivative of $ y(x) = 4 + \sin(2) $ is:
$$
\frac{dy}{dx} = 0
$$

---

4. $ y(x) = 2x^3 - 3x^2 + 8x -9 $

To compute the derivative of $$ y(x) = 2x^3 - 3x^2 + 8x - 9 $$, we use standard derivative rules.

### Step 1: Apply the power rule
The power rule states:
$$
\frac{d}{dx}[x^n] = n x^{n-1}
$$
and the derivative of a constant is $ 0 $.

### Step 2: Compute the derivative term by term
$
y(x) = 2x^3 - 3x^2 + 8x - 9
$

1. Derivative of $ 2x^3 $: 
$
\frac{d}{dx}[2x^3] = 6x^2
$
2. Derivative of $ -3x^2 $: 
$
\frac{d}{dx}[-3x^2] = -6x
$
3. Derivative of $ 8x $: 
$
\frac{d}{dx}[8x] = 8
$
4. Derivative of $ -9 $: 
$
\frac{d}{dx}[-9] = 0
$

### Step 3: Combine the results
$
\frac{dy}{dx} = 6x^2 - 6x + 8
$

### Final Answer
The derivative of $ y(x) = 2x^3 - 3x^2 + 8x - 9 $ is:
$$
\frac{dy}{dx} = 6x^2 - 6x + 8
$$

---

5. $$ y(x) = 6x^{1/3}$$

To compute the derivative of $ y(x) = 6x^{1/3} $, we use the **power rule**.

### Step 1: Apply the power rule
The power rule states:
$
\frac{d}{dx}[x^n] = n x^{n-1}
$

Here, $ n = \frac{1}{3} $.

### Step 2: Compute the derivative
$$
\frac{dy}{dx} = 6 \cdot \frac{1}{3} x^{\frac{1}{3} - 1}
$$

Simplify:
$$
\frac{dy}{dx} = 2x^{-\frac{2}{3}}
$$

### Step 3: Express the answer in a simplified form
Using the negative exponent rule ($ x^{-n} = \frac{1}{x^n} $):
$$
\frac{dy}{dx} = \frac{2}{x^{\frac{2}{3}}}
$$

### Final Answer
The derivative of $$ y(x) = 6x^{1/3} $$ is:
$$
\frac{dy}{dx} = \frac{2}{x^{2/3}}
$$

---

6. $y(x) = \sqrt x$

To compute the derivative of $ y(x) = x $, we use the **power rule**.

### Step 1: Apply the power rule
The power rule states:
$$
\frac{d}{dx}[x^n] = n x^{n-1}
$$

Here, $ n = 1 $. 

### Step 2: Compute the derivative
$$
\frac{dy}{dx} = 1 \cdot x^{1-1} = x^0 = 1
$$

### Final Answer
The derivative of $ y(x) = x $ is:
$$
\frac{dy}{dx} = 1
$$

---

7. $y(x) = cos(x) + sin(x)$

To compute the derivative of $$ y(x) = \cos(x) + \sin(x) $$, we use the standard derivative rules for trigonometric functions:

### Step 1: Derivative rules for sine and cosine
- The derivative of $ \cos(x) $ is $ -\sin(x) $.
- The derivative of $ \sin(x) $ is $ \cos(x) $.

### Step 2: Compute the derivative
$$
\frac{dy}{dx} = \frac{d}{dx}[\cos(x)] + \frac{d}{dx}[\sin(x)]
$$
$$
\frac{dy}{dx} = -\sin(x) + \cos(x)
$$

### Final Answer
The derivative of $ y(x) = \cos(x) + \sin(x) $ is:
$$
\frac{dy}{dx} = -\sin(x) + \cos(x)
$$

---

8. $$ y(x) = 2 cos(x) sin(x) $$

To compute the derivative of $ y(x) = 2\sin(x)\cos(x) $, we can use the **product rule** and **trigonometric identities**.

---

### Step 1: Recall the product rule
The product rule states:
$
\frac{d}{dx}[u \cdot v] = u'v + uv'
$
Here, $ u = \sin(x) $ and $ v = \cos(x) $.

---

### Step 2: Differentiate using the product rule
1. Compute $$ u' = \frac{d}{dx}[\sin(x)] = \cos(x) $$.
2. Compute $$ v' = \frac{d}{dx}[\cos(x)] = -\sin(x) $$.

Now apply the product rule:
$$
\frac{dy}{dx} = 2  \cos(x)\cos(x)
$$

Simplify:
$$
\frac{dy}{dx} = 2  \cos^2(x) 
$$

---

### Step 3: Simplify using a trigonometric identity
The expression $ \cos^2(x) - \sin^2(x) $ is equivalent to $ \cos(2x) $ (a standard double-angle identity).

Thus:
$$
\frac{dy}{dx} = 2\cos(2x)
$$

---

### Final Answer
The derivative of $$ y(x) = 2\sin(x)\cos(x) $$ is:
$$
\frac{dy}{dx} = 2\cos(2x)
$$

----

9. $$y(x) = xsinx$$

To compute the derivative of $ y(x) = x \sin(x) $, we use the **product rule**.

---

### Step 1: Recall the product rule
The product rule states:
$
\frac{d}{dx}[u \cdot v] = u'v + uv'
$
Here:
- $ u = x $
- $ v = \sin(x) $)

---

### Step 2: Compute derivatives of $ u $ and $ v $
1. $$ u' = \frac{d}{dx}[x] = 1 $$
2. $$ v' = \frac{d}{dx}[\sin(x)] = \cos(x) $$

---

### Step 3: Apply the product rule
$$
\frac{dy}{dx} = u'v + uv' = (1)(\sin(x)) + (x)(\cos(x))
$$

Simplify:
$$
\frac{dy}{dx} = \sin(x) + x\cos(x)
$$

---

### Final Answer
The derivative of $ y(x) = x \sin(x) $ is:
$$
\frac{dy}{dx} = \sin(x) + x\cos(x)
$$

---

10. $$y(x) = (x + 1)(x+1)$$

To compute the derivative of $ y(x) = (x + 1)(x + 1) $, we first recognize that the expression is a square of $(x + 1) $. We can simplify it as:

$
y(x) = (x + 1)^2
$

Now, we'll differentiate using the **chain rule**.

---

### Step 1: Apply the chain rule
The chain rule states that the derivative of $ (u(x))^n $ is $ n \cdot (u(x))^{n-1} \cdot u'(x) $, where $ u(x) = x + 1 $ and $ n = 2 $.

### Step 2: Differentiate
First, differentiate $ u(x) = x + 1 $:
$$
u'(x) = 1
$$

Now, apply the chain rule:
$$
\frac{dy}{dx} = 2(x + 1) \cdot 1
$$
Simplifying:
$$
\frac{dy}{dx} = 2(x + 1)
$$

---

### Final Answer
The derivative of $$ y(x) = (x + 1)(x + 1) $$ is:
$$
\frac{dy}{dx} = 2(x + 1)
$$

---

11. $$ y(x) =  \frac {x}{x+1}$$

---

To compute the derivative of $ y(x) = \frac{x}{x + 1} $, we will apply the **quotient rule**.

### Step 1: Recall the quotient rule
For a function $ y(x) = \frac{u(x)}{v(x)} $, the quotient rule is:
$
\frac{dy}{dx} = \frac{u'(x)v(x) - u(x)v'(x)}{[v(x)]^2}
$
Here:
- $ u(x) = x $
- $v(x) = x + 1 $

### Step 2: Compute the derivatives of $ u(x) $ and $ v(x) $
1. $$ u'(x) = \frac{d}{dx}[x] = 1 $$
2. $$ v'(x) = \frac{d}{dx}[x + 1] = 1 $$

### Step 3: Apply the quotient rule
$$
\frac{dy}{dx} = \frac{(1)(x + 1) - (x)(1)}{(x + 1)^2}
$$

Simplify the numerator:
$$
\frac{dy}{dx} = \frac{x + 1 - x}{(x + 1)^2} = \frac{1}{(x + 1)^2}
$$

### Final Answer
The derivative of $ y(x) = \frac{x}{x + 1} $ is:
$$
\frac{dy}{dx} = \frac{1}{(x + 1)^2}
$$

---
12. $$ y(x) = (x+1) exp(x)$$

To compute the derivative of $$ y(x) = (x + 1) \exp(x) $$, we use the **product rule**.

### Step 1: Recall the product rule
The product rule states:
$$
\frac{d}{dx}[u(x) \cdot v(x)] = u'(x)v(x) + u(x)v'(x)
$$
Here:
- $$ u(x) = x + 1 $$
- $$ v(x) = \exp(x) $$

### Step 2: Compute derivatives of $ u(x) $ and $ v(x) $
1. $$ u'(x) = \frac{d}{dx}[x + 1] = 1 $$
2. $$ v'(x) = \frac{d}{dx}[\exp(x)] = \exp(x) $$

### Step 3: Apply the product rule
$$
\frac{dy}{dx} = (1)(\exp(x)) + (x + 1)(\exp(x))
$$

Simplify:
$$
\frac{dy}{dx} = \exp(x) + (x + 1) \exp(x)
$$

Factor out $ \exp(x) $:
$$
\frac{dy}{dx} = \exp(x)(1 + x + 1)
$$
$$
\frac{dy}{dx} = \exp(x)(x + 2)
$$

### Final Answer
The derivative of $$ y(x) = (x + 1) \exp(x) $$ is:
$$
\frac{dy}{dx} = \exp(x)(x + 2)
$$

---

13. $$ y(x) = sin(x^2)$$

To compute the derivative of $$ y(x) = \sin(x^2) $$, we use the **chain rule**.

### Step 1: Recall the chain rule
The chain rule states that if $ y(x) = \sin(u(x)) $, then:
$$
\frac{dy}{dx} = \cos(u(x)) \cdot u'(x)
$$
In this case, $ u(x) = x^2 $

### Step 2: Compute the derivative of $ u(x) = x^2 $
$$
u'(x) = \frac{d}{dx}[x^2] = 2x
$$

### Step 3: Apply the chain rule
$$
\frac{dy}{dx} = \cos(x^2) \cdot 2x
$$

### Final Answer
The derivative of $$ y(x) = \sin(x^2) $$ is:
$$
\frac{dy}{dx} = 2x \cos(x^2)
$$
----

$$y(x) = exp(-2x)$$

To compute the derivative of $$ y(x) = \exp(-2x) $$, we apply the **chain rule**.

### Step 1: Recall the chain rule
The chain rule states that if $$ y(x) = \exp(u(x)) $$, then:
$$
\frac{dy}{dx} = \exp(u(x)) \cdot u'(x)
$$
Here, $ u(x) = -2x $.

### Step 2: Compute the derivative of $ u(x) = -2x $
$$
u'(x) = \frac{d}{dx}[-2x] = -2
$$

### Step 3: Apply the chain rule
$$
\frac{dy}{dx} = \exp(-2x) \cdot (-2)
$$

### Final Answer
The derivative of $ y(x) = \exp(-2x) $ is:
$$
\frac{dy}{dx} = -2 \exp(-2x)
$$

---

$$ y(x) =  \frac {x}{sin(x+1)} $$

To compute the derivative of $$ y(x) = \frac{x}{\sin(x + 1)} $$, we use the **quotient rule**.

---

### Step 1: Recall the quotient rule
The quotient rule states:
$$
\frac{dy}{dx} = \frac{u'(x)v(x) - u(x)v'(x)}{[v(x)]^2}
$$
Here:
- $ u(x) = x $
- $ v(x) = \sin(x + 1) $

---

### Step 2: Compute derivatives of $ u(x) $ and $ v(x) $
1. $$ u'(x) = \frac{d}{dx}[x] = 1 $$
2. $$ v'(x) = \frac{d}{dx}[\sin(x + 1)] = \cos(x + 1) \cdot \frac{d}{dx}[x + 1] = \cos(x + 1) \cdot 1 = \cos(x + 1) $$

---

### Step 3: Apply the quotient rule
$$
\frac{dy}{dx} = \frac{(1)(\sin(x + 1)) - (x)(\cos(x + 1))}{[\sin(x + 1)]^2}
$$

Simplify the numerator:
$$
\frac{dy}{dx} = \frac{\sin(x + 1) - x \cos(x + 1)}{[\sin(x + 1)]^2}
$$

---

### Final Answer
The derivative of $$ y(x) = \frac{x}{\sin(x + 1)} $$ is:
$$
\frac{dy}{dx} = \frac{\sin(x + 1) - x \cos(x + 1)}{[\sin(x + 1)]^2}
$$
---

$$ y(x) = \sqrt {2x + 1} $$

To compute the derivative of $ y(x) = \sqrt{2x + 1} $, we rewrite the square root in exponential form and then use the **chain rule**.

---

### Step 1: Rewrite the function
$$
y(x) = (2x + 1)^{1/2}
$$

---

### Step 2: Apply the chain rule
The chain rule states:
$$
\frac{d}{dx} \left[ (u(x))^n \right] = n \cdot (u(x))^{n-1} \cdot u'(x)
$$
Here:
- $ u(x) = 2x + 1 $
- $ n = \frac{1}{2} $

---

### Step 3: Compute the derivative
First, compute $$ u'(x) = \frac{d}{dx}[2x + 1] = 2 $$.

Now, apply the chain rule:
$$
\frac{dy}{dx} = \frac{1}{2} (2x + 1)^{-1/2} \cdot 2
$$

Simplify:
$$
\frac{dy}{dx} = \frac{2}{2} (2x + 1)^{-1/2}
$$
$$
\frac{dy}{dx} = (2x + 1)^{-1/2}
$$

Rewrite in terms of the square root:
$$
\frac{dy}{dx} = \frac{1}{\sqrt{2x + 1}}
$$

---

### Final Answer
The derivative of $$ y(x) = \sqrt{2x + 1} $$ is:
$$
\frac{dy}{dx} = \frac{1}{\sqrt{2x + 1}}
$$

2. Prove

$$ \frac {d}{dx} (ln(sin(x))) = cos(x)